ptr_cmp wip

progs64/verif_ptr_cmp.v
@@ -4,6 +4,10 @@ Require Import VST.progs64.ptr_cmp.
 #[export] Instance CompSpecs : compspecs. make_compspecs prog. Defined.
 Definition Vprog : varspecs. mk_varspecs prog. Defined.
 
+Section Spec.
+
+Context  `{!default_VSTGS Σ}.
+
 Definition t_struct_tree := Tstruct _tree noattr.
 
 (** Some useful lemmas about comparing two pointers. 
@@ -17,43 +21,42 @@ Inductive Tree : Type :=
 Fixpoint tree_rep (t: Tree) (p p_lch p_rch: val): mpred :=
   match t with
   | T k lch rch   =>
-    EX p_lch_l: val, EX p_lch_r: val, 
-    EX p_rch_l: val, EX p_rch_r: val, 
+    ∃ (p_lch_l p_lch_r p_rch_l p_rch_r: val),
     data_at Tsh t_struct_tree 
       (Vint (Int.repr k), (p_lch, p_rch)) p
-    * tree_rep lch p_lch p_lch_l p_lch_r 
-    * tree_rep rch p_rch p_rch_l p_rch_r 
-  | E => !! (p = nullval) && emp 
+    ∗ tree_rep lch p_lch p_lch_l p_lch_r 
+    ∗ tree_rep rch p_rch p_rch_l p_rch_r 
+  | E => ⌜p = nullval⌝ ∧ emp 
   end.
 
 (** Representation of the parent-child relationship. *)
 Definition fa_rep (d: bool) (t: Tree) (p_ch p_fa: val) : mpred :=
   match d with
   | true    => 
-    EX p_oppo: val, tree_rep t p_fa p_ch p_oppo
+    ∃ p_oppo: val, tree_rep t p_fa p_ch p_oppo
   | false   =>
-    EX p_oppo: val, tree_rep t p_fa p_oppo p_ch
+    ∃ p_oppo: val, tree_rep t p_fa p_oppo p_ch
   end.
 
 (** Some basic lemmas. *)
 Lemma tree_rep_saturate_local:
-   forall t p p_lch p_rch, tree_rep t p p_lch p_rch |-- !! is_pointer_or_null p.
+   forall t p p_lch p_rch, tree_rep t p p_lch p_rch ⊢ ⌜is_pointer_or_null p⌝.
 Proof.
   destruct t; simpl; intros.
   entailer!.
   Intros p_lch_l p_lch_r p_rch_l p_rch_r. entailer!.
 Qed.
-#[export] Hint Resolve tree_rep_saturate_local: saturate_local.
+Hint Resolve tree_rep_saturate_local: saturate_local.
 
 Lemma tree_rep_valid_pointer:
-  forall t p p_lch p_rch, tree_rep t p p_lch p_rch |-- valid_pointer p.
+  forall t p p_lch p_rch, tree_rep t p p_lch p_rch ⊢ valid_pointer p.
 Proof.
   intros.
   destruct t. 
   - simpl. entailer!. 
   - simpl; normalize; auto with valid_pointer.
 Qed.
-#[export] Hint Resolve tree_rep_valid_pointer: valid_pointer.
+Hint Resolve tree_rep_valid_pointer: valid_pointer.
 
 Definition bool2int (d: bool) : Z :=
   match d with
@@ -79,7 +82,7 @@ Definition Gprog : funspecs :=
   ltac:(with_library prog [get_branch_spec]).
 
 (** Now try to prove this program. *)
-Theorem body_get_branch_old_fashion: semax_body Vprog Gprog f_get_branch get_branch_spec.
+Theorem body_get_branch_old_fashion: semax_body Vprog Gprog ⊤ f_get_branch get_branch_spec.
 Proof.
   start_function. 
   (* first eliminate the possibility that t is empty *)
@@ -127,8 +130,89 @@ Proof.
       (data_at_conflict Tsh t_struct_tree 
         (Vint (Int.repr k0), (p_lch_l, p_lch_r))
         (Vint (Int.repr k1), (p_rch_l, p_rch_r))
-        p_oppo top_share_nonidentity).
-      sep_apply H1.
+        p_oppo Share.nontrivial).
+        unfold POSTCONDITION. unfold abbreviate.
+        
+        (* sep_apply H1. *)
+        (* new_sep_apply H1 sep_apply_evar_tac sep_apply_prop_tac. *)
+        (* new_sep_apply_in_semax H1 sep_apply_evar_tac sep_apply_prop_tac. *)
+        eapply semax_pre(*_bupd*).
+        (* new_sep_apply_in_lifted_entailment H evar_tac prop_tac. *)
+        apply SEP_entail'.
+
+  (* go_lower; *)
+  clear_Delta_specs;
+intros;
+match goal with
+ | |- local _ ∧ PROPx _ (LOCALx _ (SEPx ?R)) ⊢ _ => check_mpreds R
+ | |- ENTAIL _, PROPx _ (LOCALx _ (SEPx ?R)) ⊢ _ => check_mpreds R
+ | |- ENTAIL _, _ ⊢ _ => fail 10 "The left-hand-side of your entailment is not in PROP/LOCAL/SEP form"
+ | _ => fail 10 "go_lower requires a proof goal in the form of (ENTAIL _ , _ ⊢ _)"
+end.
+(* clean_LOCAL_canon_mix. *)
+eapply_clean_LOCAL_right_spec;
+[solve_all_legal_glob_ident | prove_local2ptree | 
+(* solve_clean_LOCAL_right *)
+ | simpl_app_localdefs_tc].
+ let TT1 := fresh "T1" in 
+ let TT2 := fresh "T2" in
+ let ggv := fresh "GV" in
+ match goal with 
+ | |- clean_LOCAL_right Delta ?T1 ?T2 ?GV ?ass ?mp =>
+ pose T1 as TT1; pose T2 as TT2; pose GV as ggv
+ end.
+
+ pose proof (clean_LOCAL_right_sep_lift Delta T1 T2 None).
+ unfold T1, T2 in H2.
+ Search embed liftx.
+ apply H2. 
+ (* solve_clean_LOCAL_right. *)
+
+
+
+
+repeat (simple apply derives_extract_PROP; intro_PROP);
+let rho := fresh "rho" in
+split => rho;
+first
+[ simple apply quick_finish_lower
+|          
+ (let TC := fresh "TC" in apply finish_lower; intros TC ||
+ match goal with
+ | |- (_ ∧ PROPx nil _) _ ⊢ _ => fail 1 "LOCAL part of precondition is not a concrete list (or maybe Delta is not concrete)"
+ | |- _ => fail 1 "PROP part of precondition is not a concrete list"
+ end);
+cbv [fold_right_sepcon];
+unfold_for_go_lower;
+simpl tc_val;
+cbv [typecheck_exprlist typecheck_expr]; simpl tc_andp;
+simpl msubst_denote_tc_assert;
+try monPred.unseal; unfold monPred_at;
+try clear dependent rho;
+clear_Delta;
+rewrite ?bi.sep_emp
+].
+
+
+  match goal with |- ?R ⊢ ?R2 =>
+    let r2 := fresh "R2" in pose (r2 := R2); change (R ⊢ r2);
+    new_sep_apply_in_entailment H evar_tac prop_tac; [ .. |
+    match goal with |- ?R' ⊢ _ =>
+      let R'' := refold_right_sepcon R' in
+      replace R' with (fold_right_sepcon R'')
+             by (unfold fold_right_sepcon; rewrite ?bi.sep_emp; reflexivity);
+          subst r2; apply derives_refl
+    end]
+  end.
+
+
+        lazymatch goal with
+  | |- ENTAIL _ , _ ⊢ _ => eapply ENTAIL_trans; [new_sep_apply_in_lifted_entailment H1 sep_apply_evar_tac sep_apply_prop_tac | ]
+  | |- _ ⊢ _ => new_sep_apply_in_entailment H1 sep_apply_evar_tac sep_apply_prop_tac
+  | |- semax _ _ _ _ _ => new_sep_apply_in_semax H1 sep_apply_evar_tac sep_apply_prop_tac
+  end.
+
+      
       sep_apply FF_local_facts.
       Intros.
       destruct H2.
